examples/low-level/FStar.Format.fst
@@ -1,0 +1,230 @@
+module FStar.Format
+
+open FStar.Ghost
+open FStar.UInt8
+open FStar.UInt32
+open FStar.Int.Cast
+open FStar.Seq
+open FStar.ImmBuffer
+
+type lsize = n:int{n = 1 \/ n = 2 \/ n = 3}
+type csize = n:t{v n = 1 \/ v n = 2 \/ v n = 3}
+
+val read_length: 
+  b:buffer u8 -> 
+  n:csize{v n <= length b} -> 
+  Tot UInt32.t
+let read_length b n =
+  if n = 1ul then (
+    let b0 = read b 0ul in
+    uint8_to_uint32 b0
+  ) else if n = 2ul then (
+    let b1 = read b 0ul in
+    let b0 = read b 1ul in
+    let b0 = uint8_to_uint32 b0 in
+    let b1 = uint8_to_uint32 b1 in
+    b0 |^ (b1 <<^ 8ul)
+  ) else (
+    let b2 = read b 0ul in
+    let b1 = read b 1ul in
+    let b0 = read b 2ul in
+    let b0 = uint8_to_uint32 b0 in
+    let b1 = uint8_to_uint32 b1 in
+    let b2 = uint8_to_uint32 b2 in
+    b0 |^ (b1 <<^ 8ul) |^ (b2 <<^ 16ul)
+  )
+
+let vlbytes (n:lsize) = b:buffer u8{length b >= n /\ length b = n + v (read_length b (uint_to_t n))}
+
+val vlparse: b:buffer u8 -> n:csize -> len:UInt32.t{v len < length b} -> Tot (result (vlbytes (v n)))
+let vlparse b n len =
+  if n >^ len then Error "Too short"
+  else 
+    let l = read_length b n in
+    if length b < v n + v l then Error "Wrong vlbytes format"
+    else (
+      let b' = sub b 0ul (n +^ l) in
+      Correct b'
+    )
+
+#set-options "--lax"
+
+val vlsplit: b:buffer u8 -> n:csize -> len:UInt32.t{v len < length b} ->
+  Tot (result (vlbytes (v n) * buffer u8))
+let vlsplit b n len =
+  if n >^ len then Error "Too short"
+  else 
+    let l = read_length b n in
+    assume (v l + v n < pow2 32);
+    if len <^ n +^ l then Error "Wrong vlbytes format"
+    else (
+      let b' = sub b 0ul (n +^ l) in
+      let b'' = offset b (n +^ l) in
+      Correct (b', b'') 
+    )
+
+val lemma_vlsplit: b:buffer u8 -> n:csize -> len:UInt32.t{v len < length b} ->
+  Lemma 
+    (requires (is_Correct (vlsplit b n len)))
+    (ensures  (let t = vlsplit b n len in 
+      (is_Correct t /\ (let t = correct t in 
+	Seq.append (as_seq (fst t)) (as_seq (snd t)) == as_seq b))))
+let lemma_vlsplit b n = admit() // TODO
+
+type buf (#ty:sizeof_t) (t:serializable ty) (n:lsize) = b:buffer t{length b = n}
+
+(* let vlbuf (#ty:sizeof_t) (n:lsize) (t:serializable t) = *)
+(*   (l:buffer u8{length l = n} &  b:buffer t{length b = v (read_length l (uint_to_t n))}) *)
+
+let vlbuf (#ty:sizeof_t) (n:lsize) (t:serializable ty) =
+  b:buffer u8{length b >= n
+    /\ (let content = Seq.slice (as_seq_bytes b) n (bytes_length b) in
+      
+      Seq.length content % sizeof ty = 0 /\ is_Correct (of_seq_bytes #ty #t content))}
+
+assume val vlbuf_parse: #ty:sizeof_t -> t:serializable ty -> b:buffer u8 -> n:csize{length b >= v n} -> 
+  Tot (result (vlbuf (v n) t))
+
+assume val vlbuf_split: #ty:sizeof_t -> t:serializable ty -> b:buffer u8 -> n:csize{length b >= v n} -> 
+  Tot (result (vlbuf (v n) t * buffer u8))
+
+assume BufHasSize: forall (#ty:sizeof_t) (t:serializable ty) (n:lsize).
+  hasSize (buf #ty t n) /\ sizeof (buf #ty t n) = sizeof (buffer t)
+
+assume VlbytesHasSize: forall (n:lsize).
+  hasSize (vlbytes n) /\ sizeof (vlbytes n) = sizeof (buffer u8)
+
+assume VlbufHasSize: forall (#ty:sizeof_t) (t:serializable ty) (n:lsize).
+  hasSize (vlbuf #ty n t) /\ sizeof (vlbuf #ty n t) = sizeof (buffer t)
+
+assume val serialize_ptr: serializer bytes
+assume val parse_ptr: parser serialize_ptr
+
+noeq type key_share = {
+  ks_group_name: buf u16 1;
+  ks_public_key: vlbytes 2
+}
+
+assume KeyShareHasSize: 
+  hasSize key_share /\ sizeof key_share = sizeof (buf u16 1) + sizeof (vlbytes 2)
+
+let serialize_key_share: serializer key_share =
+  admit();
+  fun (ks:key_share) ->
+    serialize_ptr ks.ks_group_name @| serialize_ptr ks.ks_public_key
+
+#set-options "--lax"
+
+let parse_key_share_bytes (b:bytes) (len:UInt32.t) : Tot (result key_share) =
+  if len <^ 4ul then Error "Too short"
+  else let ks_group_name = cast u16 u8 (sub (to_buffer u8 b) 0ul 2ul) in
+       let ks_public_key = offset (to_buffer u8 b) 2ul in       
+       match vlparse ks_public_key 2ul (len -^ 2ul) with
+       | Correct x ->
+	 Correct ({ks_group_name = ks_group_name; ks_public_key = x})
+       | Error z -> Error z
+
+let parse_key_share: parser serialize_key_share = fun s ->
+  if Seq.length <> sizeof key_share then Error "Wrong pointer value"
+  else (
+    match parse_ptr with
+    | Correct x ->  
+    | Error z
+  )
+
+let key_share_bytes (ks:key_share) : Tot (seq byte) =
+  as_seq_bytes (to_bytes ks.ks_group_name) @| as_seq_bytes (to_bytes ks.ks_public_key)
+
+let key_share' = Serializable key_share seri
+
+let key_share_ext = vlbuf 2 key_share
+
+let parse_key_share_ext_bytes (kse:key_share_ext) =
+  let 
+
+noeq type client_extension =
+ | CE_extended_ms
+ | CE_secure_renegotiation of buf_var 1 u8
+ | CE_supported_groups of buf_var 2 u16
+ | CE_supported_point_formats of buf_var 1 u8
+ | CE_signature_algorithms of buf_var 2 u16
+ | CE_earlyData
+ | CE_keyShare of arraybuf_var 2 key_share
+ | CE_preSharedKey of arraybuf_var 2 (buf_var 2 u8)
+ | CE_server_names of arraybuf_var 2 (buf_var 2 u8)
+
+type ch =  {
+  ch_protocol_version:buf u16 1;
+  ch_client_random:buf u8 32;
+  ch_sessionID:buf_var 1 u8;
+  ch_cipher_suites:buf_var 2 u16;
+  ch_compressions:buf_var 1 u8;
+  ch_extensions:arraybuf_var 2 client_extension;
+}
+
+
+(* type c_extensions = { *)
+(*   ce_extended_ms: byte; *)
+(*   ce_secure_renegotiation: buf_var 1 1; *)
+(*   ce_supported_groups: buf_var 2 2; *)
+(*   ce_supported_point_formats: buf_var 1 1; *)
+(*   ce_signature_algorithms: buf_var 2 2; *)
+(*   ce_earlyData: byte; *)
+(*   ce_keyShare: key_share *)
+(*   ce_preSharedKey: arraybuf_var 2 (buf_var 2 1) *)
+(*   ce_server_names: arraybuf_var 2 (buf_var 2 1) *)
+(* } *)
+
+(* type c_hello = { *)
+(*   c_protocol_version:buf 2 1; *)
+(*   c_client_random:buf 1 32; *)
+(*   ch_sessionID:buf_var 1 1; *)
+(*   ch_cipher_suites:buf_var 2 2; *)
+(*   ch_compressions:buf_var 1 1; *)
+(*   ch_extensions:arraybuf_var 2 client_extension; *)
+(* } *)
+
+(*
+let clientHelloBytes ch buf = ...
+  
+  *)
+
+type server_extension =
+ | SE_extended_ms
+ | SE_secure_renegotiation of buf_var 1 u8
+ | SE_supported_point_formats of buf_var 1 u8
+ | SE_earlyData
+ | SE_keyShare of key_share
+ | SE_preSharedKey of buf_var 2 u8
+ | SE_server_names
+
+type sh =  {
+  sh_protocol_version:buf u16 1;
+  sh_client_random:buf u8 32;
+  sh_sessionID:option (buf_var 1 u8);
+  sh_cipher_suites:buf_var 2 u16;
+  sh_compressions:option (buf_var 1 u8);
+  sh_extensions:arraybuf_var 2 server_extension;
+}
+
+(*
+struct
+{ version : buf 1 short;
+  random:   buf 32 short;
+  sessionid: buf_var 1 byte;
+  ciphersuites: buf_var 2 short;
+  compressions: buf_var 1 byte;
+  extensions:   buf_var 2
+    struct {
+      name: buf 1 short;
+      payload: buf_var 2
+         union {
+  	   empty;
+	   buf_var 1 bytte;
+	   |
+      list <struct [buf 2 1; buf_var 2 1]>
+            
+    >
+   >
+  ]
+*)
